src/benchmark.v
@@ -1,7 +1,7 @@
 From stdpp Require Import base.
 From Stdlib Require Import Uint63.
 From Stdlib Require Import Array.PArray.
-From marble Require Import list_init.
+From listz Require Import listz.
 From marble Require Import bool int array compare sort vector.
 From marble Require Import compare.
 
