src/vector.v
@@ -1,7 +1,8 @@
 From stdpp Require Import numbers list.
 From Stdlib Require Import Uint63.
 From Stdlib Require Import Array.PArray.
-From marble Require Import tactics list_extra bool iteration int wp wp_tactics array.
+From listz Require Import listz.
+From marble Require Import tactics bool iteration int wp wp_tactics array.
 Implicit Types _i _j _k _n : int.
 
 Unset Universe Minimization ToSet.
